NonEmpty/ArrayCorrectByConstruction.lean
@@ -2,4 +2,7 @@ module
 
 prelude
 public import NonEmpty.ArrayCorrectByConstruction.Basic
+public import NonEmpty.ArrayCorrectByConstruction.Ops
+public import NonEmpty.ArrayCorrectByConstruction.Instances
+public import NonEmpty.ArrayCorrectByConstruction.Notation
 public import NonEmpty.ArrayCorrectByConstruction.ToExpr
