NonEmpty/ListCorrectByConstruction.lean
@@ -2,4 +2,7 @@ module
 
 prelude
 public import NonEmpty.ListCorrectByConstruction.Basic
+public import NonEmpty.ListCorrectByConstruction.Ops
+public import NonEmpty.ListCorrectByConstruction.Instances
+public import NonEmpty.ListCorrectByConstruction.Notation
 public import NonEmpty.ListCorrectByConstruction.ToExpr
