NonEmpty/String/Intercalate/ArrayCorrectByConstruction.lean
@@ -2,6 +2,9 @@ module
 
 public import NonEmpty.String.Basic
 public import NonEmpty.ArrayCorrectByConstruction.Basic
+public import NonEmpty.ArrayCorrectByConstruction.Ops
+public import NonEmpty.ArrayCorrectByConstruction.Instances
+public import NonEmpty.ArrayCorrectByConstruction.Notation
 
 @[expose] public section
 
